move to a one-field structure

src/Std/Data/ExtDTreeMap/Basic.lean
@@ -71,14 +71,52 @@ be used in nested inductive types. For these use cases, `Std.DTreeMap.Raw` and
 `Std.DTreeMap.Raw.WF` unbundle the invariant from the tree map. When in doubt, prefer
 `ExtDTreeMap` over `DTreeMap.Raw`.
 -/
-def ExtDTreeMap (α : Type u) (β : α → Type v) (cmp : α → α → Ordering := by exact compare) :=
-  Quotient (DTreeMap.isSetoid α β cmp)
+structure ExtDTreeMap (α : Type u) (β : α → Type v) (cmp : α → α → Ordering := by exact compare) where
+  /-- Implementation detail of the tree map -/
+  mk' ::
+  /-- Implementation detail of the tree map -/
+  inner : Quotient (DTreeMap.isSetoid α β cmp)
+
+/-- Implementation detail of the tree map -/
+abbrev ExtDTreeMap.mk (t : DTreeMap α β cmp) : ExtDTreeMap α β cmp :=
+  .mk' (Quotient.mk _ t)
+
+/-- Implementation detail of the tree map -/
+abbrev ExtDTreeMap.lift {γ : Sort w} (f : DTreeMap α β cmp → γ) (h : ∀ a b, a ~m b → f a = f b)
+    (t : ExtDTreeMap α β cmp) : γ :=
+  t.1.lift f h
+
+/-- Implementation detail of the tree map -/
+abbrev ExtDTreeMap.liftOn₂ {γ : Sort w} (t₁ t₂ : ExtDTreeMap α β cmp)
+    (f : DTreeMap α β cmp → DTreeMap α β cmp → γ) (h : ∀ a b c d, a ~m c → b ~m d → f a b = f c d) : γ :=
+  t₁.1.liftOn₂ t₂.1 f h
+
+/-- Implementation detail of the tree map -/
+abbrev ExtDTreeMap.pliftOn {γ : Sort w} (t : ExtDTreeMap α β cmp)
+    (f : (x : DTreeMap α β cmp) → t = mk x → γ) (h : ∀ a b h₁ h₂, a ~m b → f a h₁ = f b h₂) : γ :=
+  t.1.pliftOn (fun x hx => f x (by cases t; cases hx; rfl)) (fun a b _ _ h' => h a b _ _ h')
+
+theorem ExtDTreeMap.sound {t₁ t₂ : DTreeMap α β cmp} (h : t₁ ~m t₂) : mk t₁ = mk t₂ :=
+  congrArg mk' (Quotient.sound h)
+
+theorem ExtDTreeMap.exact {t₁ t₂ : DTreeMap α β cmp} (h : mk t₁ = mk t₂) : t₁ ~m t₂ :=
+  Quotient.exact (congrArg inner h)
+
+@[cases_eliminator, induction_eliminator, elab_as_elim]
+theorem ExtDTreeMap.inductionOn {motive : ExtDTreeMap α β cmp → Prop}
+    (t : ExtDTreeMap α β cmp) (mk : ∀ a, motive (mk a)) : motive t :=
+  (t.1.inductionOn fun _ => mk _ : motive ⟨t.1⟩)
+
+@[elab_as_elim]
+theorem ExtDTreeMap.inductionOn₂ {motive : ExtDTreeMap α β cmp → ExtDTreeMap α β cmp → Prop}
+    (t₁ t₂ : ExtDTreeMap α β cmp) (mk : ∀ a b, motive (mk a) (mk b)) : motive t₁ t₂ :=
+  t₁.inductionOn fun _ => t₂.inductionOn fun _ => mk _ _
 
 namespace ExtDTreeMap
 
 @[inline, inherit_doc DTreeMap.empty]
 def empty : ExtDTreeMap α β cmp :=
-  Quotient.mk' .empty
+  mk .empty
 
 instance : EmptyCollection (ExtDTreeMap α β cmp) where
   emptyCollection := empty
@@ -92,8 +130,7 @@ theorem empty_eq_emptyc : (empty : ExtDTreeMap α β cmp) = ∅ :=
 
 @[inline, inherit_doc DTreeMap.insert]
 def insert [TransCmp cmp] (t : ExtDTreeMap α β cmp) (a : α) (b : β a) : ExtDTreeMap α β cmp :=
-  t.lift (fun m => Quotient.mk' (m.insert a b))
-    (fun m m' (h : m ~m m') => Quotient.sound (h.insert a b))
+  t.lift (fun m => mk (m.insert a b)) (fun _ _ h => sound (h.insert a b))
 
 instance [TransCmp cmp] : Singleton ((a : α) × β a) (ExtDTreeMap α β cmp) where
   singleton e := (∅ : ExtDTreeMap α β cmp).insert e.1 e.2
@@ -106,41 +143,40 @@ instance [TransCmp cmp] : LawfulSingleton ((a : α) × β a) (ExtDTreeMap α β 
 
 @[inline, inherit_doc DTreeMap.insertIfNew]
 def insertIfNew [TransCmp cmp] (t : ExtDTreeMap α β cmp) (a : α) (b : β a) : ExtDTreeMap α β cmp :=
-  t.lift (fun m => Quotient.mk' (m.insertIfNew a b))
-    (fun m m' (h : m ~m m') => Quotient.sound (h.insertIfNew a b))
+  t.lift (fun m => mk (m.insertIfNew a b)) (fun _ _ h => sound (h.insertIfNew a b))
 
 @[inline, inherit_doc DTreeMap.containsThenInsert]
 def containsThenInsert [TransCmp cmp] (t : ExtDTreeMap α β cmp) (a : α) (b : β a) : Bool × ExtDTreeMap α β cmp :=
-  t.lift (fun m => let m' := m.containsThenInsert a b; (m'.1, Quotient.mk' m'.2))
-    (fun m m' (h : m ~m m') =>
+  t.lift (fun m => let m' := m.containsThenInsert a b; (m'.1, mk m'.2))
+    (fun m m' h =>
       Prod.ext
         (m.containsThenInsert_fst.symm ▸ m'.containsThenInsert_fst.symm ▸ h.contains_eq)
-        (Quotient.sound <|
+        (sound <|
           m.containsThenInsert_snd.symm ▸ m'.containsThenInsert_snd.symm ▸ h.insert a b))
 
 @[inline, inherit_doc DTreeMap.containsThenInsertIfNew]
 def containsThenInsertIfNew [TransCmp cmp] (t : ExtDTreeMap α β cmp) (a : α) (b : β a) :
     Bool × ExtDTreeMap α β cmp :=
-  t.lift (fun m => let m' := m.containsThenInsertIfNew a b; (m'.1, Quotient.mk' m'.2))
-    (fun m m' (h : m ~m m') =>
+  t.lift (fun m => let m' := m.containsThenInsertIfNew a b; (m'.1, mk m'.2))
+    (fun m m' h =>
       Prod.ext
         (m.containsThenInsertIfNew_fst.symm ▸ m'.containsThenInsertIfNew_fst.symm ▸ h.contains_eq)
-        (Quotient.sound <|
+        (sound <|
           m.containsThenInsertIfNew_snd.symm ▸ m'.containsThenInsertIfNew_snd.symm ▸ h.insertIfNew a b))
 
 @[inline, inherit_doc DTreeMap.getThenInsertIfNew?]
 def getThenInsertIfNew? [TransCmp cmp] [LawfulEqCmp cmp] (t : ExtDTreeMap α β cmp) (a : α) (b : β a) :
     Option (β a) × ExtDTreeMap α β cmp :=
-  t.lift (fun m => let m' := m.getThenInsertIfNew? a b; (m'.1, Quotient.mk' m'.2))
-    (fun m m' (h : m ~m m') =>
+  t.lift (fun m => let m' := m.getThenInsertIfNew? a b; (m'.1, mk m'.2))
+    (fun m m' h =>
       Prod.ext
         (m.getThenInsertIfNew?_fst.symm ▸ m'.getThenInsertIfNew?_fst.symm ▸ h.get?_eq)
-        (Quotient.sound <|
+        (sound <|
           m.getThenInsertIfNew?_snd.symm ▸ m'.getThenInsertIfNew?_snd.symm ▸ h.insertIfNew a b))
 
 @[inline, inherit_doc DTreeMap.contains]
 def contains [TransCmp cmp] (t : ExtDTreeMap α β cmp) (a : α) : Bool :=
-  t.lift (fun m => m.contains a) (fun m m' (h : m ~m m') => h.contains_eq)
+  t.lift (fun m => m.contains a) (fun _ _ h => h.contains_eq)
 
 instance [TransCmp cmp] : Membership α (ExtDTreeMap α β cmp) where
   mem m a := m.contains a
@@ -150,17 +186,17 @@ instance [TransCmp cmp] {m : ExtDTreeMap α β cmp} {a : α} : Decidable (a ∈ 
 
 @[inline, inherit_doc DTreeMap.size]
 def size (t : ExtDTreeMap α β cmp) : Nat :=
-  t.lift (fun m => m.size) (fun m m' (h : m ~m m') => h.size_eq)
+  t.lift (fun m => m.size) (fun _ _ h => h.size_eq)
 
 @[inline, inherit_doc DTreeMap.isEmpty]
 def isEmpty (t : ExtDTreeMap α β cmp) : Bool :=
-  t.lift (fun m => m.isEmpty) (fun m m' (h : m ~m m') => h.isEmpty_eq)
+  t.lift (fun m => m.isEmpty) (fun _ _ h => h.isEmpty_eq)
 
 @[simp, grind =]
 theorem isEmpty_iff {t : ExtDTreeMap α β cmp} [TransCmp cmp] : t.isEmpty ↔ t = ∅ := by
-  rcases t with ⟨t⟩
+  rcases t with ⟨⟨t⟩⟩
   refine t.equiv_empty_iff_isEmpty.symm.trans ?_
-  exact ⟨fun h => Quotient.sound h, Quotient.exact⟩
+  exact ⟨fun h => sound h, exact⟩
 
 @[simp]
 theorem isEmpty_eq_false_iff {t : ExtDTreeMap α β cmp} [TransCmp cmp] : t.isEmpty = false ↔ ¬t = ∅ :=
@@ -168,285 +204,285 @@ theorem isEmpty_eq_false_iff {t : ExtDTreeMap α β cmp} [TransCmp cmp] : t.isEm
 
 @[inline, inherit_doc DTreeMap.erase]
 def erase [TransCmp cmp] (t : ExtDTreeMap α β cmp) (a : α) : ExtDTreeMap α β cmp :=
-  t.lift (fun m => Quotient.mk' (m.erase a))
-    (fun m m' (h : m ~m m') => Quotient.sound (h.erase a))
+  t.lift (fun m => mk (m.erase a))
+    (fun _ _ h => sound (h.erase a))
 
 @[inline, inherit_doc DTreeMap.get?]
 def get? [TransCmp cmp] [LawfulEqCmp cmp] (t : ExtDTreeMap α β cmp) (a : α) : Option (β a) :=
-  t.lift (fun m => m.get? a) (fun m m' (h : m ~m m') => h.get?_eq)
+  t.lift (fun m => m.get? a) (fun _ _ h => h.get?_eq)
 
 @[inline, inherit_doc DTreeMap.get]
 def get [TransCmp cmp] [LawfulEqCmp cmp] (t : ExtDTreeMap α β cmp) (a : α) (h : a ∈ t) : β a :=
   t.pliftOn (fun m h' => m.get a (h' ▸ h :))
-    (fun m m' _ _ (h : m ~m m') => h.get_eq)
+    (fun _ _ _ _ h => h.get_eq)
 
 @[inline, inherit_doc DTreeMap.get!]
 def get! [TransCmp cmp] [LawfulEqCmp cmp] (t : ExtDTreeMap α β cmp) (a : α) [Inhabited (β a)] : β a :=
-  t.lift (fun m => m.get! a) (fun m m' (h : m ~m m') => h.get!_eq)
+  t.lift (fun m => m.get! a) (fun _ _ h => h.get!_eq)
 
 @[inline, inherit_doc DTreeMap.getD]
 def getD [TransCmp cmp] [LawfulEqCmp cmp] (t : ExtDTreeMap α β cmp) (a : α) (fallback : β a) : β a :=
-  t.lift (fun m => m.getD a fallback) (fun m m' (h : m ~m m') => h.getD_eq)
+  t.lift (fun m => m.getD a fallback) (fun _ _ h => h.getD_eq)
 
 @[inline, inherit_doc DTreeMap.getKey?]
 def getKey? [TransCmp cmp] (t : ExtDTreeMap α β cmp) (a : α) : Option α :=
-  t.lift (fun m => m.getKey? a) (fun m m' (h : m ~m m') => h.getKey?_eq)
+  t.lift (fun m => m.getKey? a) (fun _ _ h => h.getKey?_eq)
 
 @[inline, inherit_doc DTreeMap.getKey]
 def getKey [TransCmp cmp] (t : ExtDTreeMap α β cmp) (a : α) (h : a ∈ t) : α :=
   t.pliftOn (fun m h' => m.getKey a (h' ▸ h :))
-    (fun m m' _ _ (h : m ~m m') => h.getKey_eq)
+    (fun _ _ _ _ h => h.getKey_eq)
 
 @[inline, inherit_doc DTreeMap.getKey!]
 def getKey! [TransCmp cmp] [Inhabited α] (t : ExtDTreeMap α β cmp) (a : α) : α :=
-  t.lift (fun m => m.getKey! a) (fun m m' (h : m ~m m') => h.getKey!_eq)
+  t.lift (fun m => m.getKey! a) (fun _ _ h => h.getKey!_eq)
 
 @[inline, inherit_doc DTreeMap.getKeyD]
 def getKeyD [TransCmp cmp] (t : ExtDTreeMap α β cmp) (a : α) (fallback : α) : α :=
-  t.lift (fun m => m.getKeyD a fallback) (fun m m' (h : m ~m m') => h.getKeyD_eq)
+  t.lift (fun m => m.getKeyD a fallback) (fun _ _ h => h.getKeyD_eq)
 
 @[inline, inherit_doc DTreeMap.minEntry?]
 def minEntry? [TransCmp cmp] (t : ExtDTreeMap α β cmp) : Option ((a : α) × β a) :=
-  t.lift (fun m => m.minEntry?) (fun m m' (h : m ~m m') => h.minEntry?_eq)
+  t.lift (fun m => m.minEntry?) (fun _ _ h => h.minEntry?_eq)
 
 @[inline, inherit_doc DTreeMap.minEntry]
 def minEntry [TransCmp cmp] (t : ExtDTreeMap α β cmp) (h : t ≠ ∅) : (a : α) × β a :=
   t.pliftOn (fun m h' => m.minEntry (h' ▸ isEmpty_eq_false_iff.mpr h :))
-    (fun m m' _ _ (h : m ~m m') => h.minEntry_eq)
+    (fun _ _ _ _ h => h.minEntry_eq)
 
 @[inline, inherit_doc DTreeMap.minEntry!]
 def minEntry! [TransCmp cmp] [Inhabited ((a : α) × β a)] (t : ExtDTreeMap α β cmp) : (a : α) × β a :=
-  t.lift (fun m => m.minEntry!) (fun m m' (h : m ~m m') => h.minEntry!_eq)
+  t.lift (fun m => m.minEntry!) (fun _ _ h => h.minEntry!_eq)
 
 @[inline, inherit_doc DTreeMap.minEntryD]
 def minEntryD [TransCmp cmp] (t : ExtDTreeMap α β cmp) (fallback : (a : α) × β a) : (a : α) × β a :=
-  t.lift (fun m => m.minEntryD fallback) (fun m m' (h : m ~m m') => h.minEntryD_eq)
+  t.lift (fun m => m.minEntryD fallback) (fun _ _ h => h.minEntryD_eq)
 
 @[inline, inherit_doc DTreeMap.maxEntry?]
 def maxEntry? [TransCmp cmp] (t : ExtDTreeMap α β cmp) : Option ((a : α) × β a) :=
-  t.lift (fun m => m.maxEntry?) (fun m m' (h : m ~m m') => h.maxEntry?_eq)
+  t.lift (fun m => m.maxEntry?) (fun _ _ h => h.maxEntry?_eq)
 
 @[inline, inherit_doc DTreeMap.maxEntry]
 def maxEntry [TransCmp cmp] (t : ExtDTreeMap α β cmp) (h : t ≠ ∅) : (a : α) × β a :=
   t.pliftOn (fun m h' => m.maxEntry (h' ▸ isEmpty_eq_false_iff.mpr h :))
-    (fun m m' _ _ (h : m ~m m') => h.maxEntry_eq)
+    (fun _ _ _ _ h => h.maxEntry_eq)
 
 @[inline, inherit_doc DTreeMap.maxEntry!]
 def maxEntry! [TransCmp cmp] [Inhabited ((a : α) × β a)] (t : ExtDTreeMap α β cmp) : (a : α) × β a :=
-  t.lift (fun m => m.maxEntry!) (fun m m' (h : m ~m m') => h.maxEntry!_eq)
+  t.lift (fun m => m.maxEntry!) (fun _ _ h => h.maxEntry!_eq)
 
 @[inline, inherit_doc DTreeMap.maxEntryD]
 def maxEntryD [TransCmp cmp] (t : ExtDTreeMap α β cmp) (fallback : (a : α) × β a) : (a : α) × β a :=
-  t.lift (fun m => m.maxEntryD fallback) (fun m m' (h : m ~m m') => h.maxEntryD_eq)
+  t.lift (fun m => m.maxEntryD fallback) (fun _ _ h => h.maxEntryD_eq)
 
 @[inline, inherit_doc DTreeMap.minKey?]
 def minKey? [TransCmp cmp] (t : ExtDTreeMap α β cmp) : Option α :=
-  t.lift (fun m => m.minKey?) (fun m m' (h : m ~m m') => h.minKey?_eq)
+  t.lift (fun m => m.minKey?) (fun _ _ h => h.minKey?_eq)
 
 @[inline, inherit_doc DTreeMap.minKey]
 def minKey [TransCmp cmp] (t : ExtDTreeMap α β cmp) (h : t ≠ ∅) : α :=
   t.pliftOn (fun m h' => m.minKey (h' ▸ isEmpty_eq_false_iff.mpr h :))
-    (fun m m' _ _ (h : m ~m m') => h.minKey_eq)
+    (fun _ _ _ _ h => h.minKey_eq)
 
 @[inline, inherit_doc DTreeMap.minKey!]
 def minKey! [TransCmp cmp] [Inhabited α] (t : ExtDTreeMap α β cmp) : α :=
-  t.lift (fun m => m.minKey!) (fun m m' (h : m ~m m') => h.minKey!_eq)
+  t.lift (fun m => m.minKey!) (fun _ _ h => h.minKey!_eq)
 
 @[inline, inherit_doc DTreeMap.minKeyD]
 def minKeyD [TransCmp cmp] (t : ExtDTreeMap α β cmp) (fallback : α) : α :=
-  t.lift (fun m => m.minKeyD fallback) (fun m m' (h : m ~m m') => h.minKeyD_eq)
+  t.lift (fun m => m.minKeyD fallback) (fun _ _ h => h.minKeyD_eq)
 
 @[inline, inherit_doc DTreeMap.maxKey?]
 def maxKey? [TransCmp cmp] (t : ExtDTreeMap α β cmp) : Option α :=
-  t.lift (fun m => m.maxKey?) (fun m m' (h : m ~m m') => h.maxKey?_eq)
+  t.lift (fun m => m.maxKey?) (fun _ _ h => h.maxKey?_eq)
 
 @[inline, inherit_doc DTreeMap.maxKey]
 def maxKey [TransCmp cmp] (t : ExtDTreeMap α β cmp) (h : t ≠ ∅) : α :=
   t.pliftOn (fun m h' => m.maxKey (h' ▸ isEmpty_eq_false_iff.mpr h :))
-    (fun m m' _ _ (h : m ~m m') => h.maxKey_eq)
+    (fun _ _ _ _ h => h.maxKey_eq)
 
 @[inline, inherit_doc DTreeMap.maxKey!]
 def maxKey! [TransCmp cmp] [Inhabited α] (t : ExtDTreeMap α β cmp) : α :=
-  t.lift (fun m => m.maxKey!) (fun m m' (h : m ~m m') => h.maxKey!_eq)
+  t.lift (fun m => m.maxKey!) (fun _ _ h => h.maxKey!_eq)
 
 @[inline, inherit_doc DTreeMap.maxKeyD]
 def maxKeyD [TransCmp cmp] (t : ExtDTreeMap α β cmp) (fallback : α) : α :=
-  t.lift (fun m => m.maxKeyD fallback) (fun m m' (h : m ~m m') => h.maxKeyD_eq)
+  t.lift (fun m => m.maxKeyD fallback) (fun _ _ h => h.maxKeyD_eq)
 
 @[inline, inherit_doc DTreeMap.entryAtIdx?]
 def entryAtIdx? [TransCmp cmp] (t : ExtDTreeMap α β cmp) (n : Nat) : Option ((a : α) × β a) :=
-  t.lift (fun m => m.entryAtIdx? n) (fun m m' (h : m ~m m') => h.entryAtIdx?_eq)
+  t.lift (fun m => m.entryAtIdx? n) (fun _ _ h => h.entryAtIdx?_eq)
 
 @[inline, inherit_doc DTreeMap.entryAtIdx]
 def entryAtIdx [TransCmp cmp] (t : ExtDTreeMap α β cmp) (n : Nat) (h : n < t.size) : (a : α) × β a :=
   t.pliftOn (fun m h' => m.entryAtIdx n (h' ▸ h :))
-    (fun m m' _ _ (h : m ~m m') => h.entryAtIdx_eq)
+    (fun _ _ _ _ h => h.entryAtIdx_eq)
 
 @[inline, inherit_doc DTreeMap.entryAtIdx!]
 def entryAtIdx! [TransCmp cmp] [Inhabited ((a : α) × β a)] (t : ExtDTreeMap α β cmp) (n : Nat) : (a : α) × β a :=
-  t.lift (fun m => m.entryAtIdx! n) (fun m m' (h : m ~m m') => h.entryAtIdx!_eq)
+  t.lift (fun m => m.entryAtIdx! n) (fun _ _ h => h.entryAtIdx!_eq)
 
 @[inline, inherit_doc DTreeMap.entryAtIdxD]
 def entryAtIdxD [TransCmp cmp] (t : ExtDTreeMap α β cmp) (n : Nat)
     (fallback : (a : α) × β a) : (a : α) × β a :=
-  t.lift (fun m => m.entryAtIdxD n fallback) (fun m m' (h : m ~m m') => h.entryAtIdxD_eq)
+  t.lift (fun m => m.entryAtIdxD n fallback) (fun _ _ h => h.entryAtIdxD_eq)
 
 @[inline, inherit_doc DTreeMap.keyAtIdx?]
 def keyAtIdx? [TransCmp cmp] (t : ExtDTreeMap α β cmp) (n : Nat) : Option α :=
-  t.lift (fun m => m.keyAtIdx? n) (fun m m' (h : m ~m m') => h.keyAtIdx?_eq)
+  t.lift (fun m => m.keyAtIdx? n) (fun _ _ h => h.keyAtIdx?_eq)
 
 @[inline, inherit_doc DTreeMap.keyAtIdx]
 def keyAtIdx [TransCmp cmp] (t : ExtDTreeMap α β cmp) (n : Nat) (h : n < t.size) : α :=
   t.pliftOn (fun m h' => m.keyAtIdx n (h' ▸ h :))
-    (fun m m' _ _ (h : m ~m m') => h.keyAtIdx_eq)
+    (fun _ _ _ _ h => h.keyAtIdx_eq)
 
 @[inline, inherit_doc DTreeMap.keyAtIdx!]
 def keyAtIdx! [TransCmp cmp] [Inhabited α] (t : ExtDTreeMap α β cmp) (n : Nat) : α :=
-  t.lift (fun m => m.keyAtIdx! n) (fun m m' (h : m ~m m') => h.keyAtIdx!_eq)
+  t.lift (fun m => m.keyAtIdx! n) (fun _ _ h => h.keyAtIdx!_eq)
 
 @[inline, inherit_doc DTreeMap.keyAtIdxD]
 def keyAtIdxD [TransCmp cmp] (t : ExtDTreeMap α β cmp) (n : Nat) (fallback : α) : α :=
-  t.lift (fun m => m.keyAtIdxD n fallback) (fun m m' (h : m ~m m') => h.keyAtIdxD_eq)
+  t.lift (fun m => m.keyAtIdxD n fallback) (fun _ _ h => h.keyAtIdxD_eq)
 
 @[inline, inherit_doc DTreeMap.getEntryGE?]
 def getEntryGE? [TransCmp cmp] (t : ExtDTreeMap α β cmp) (k : α) : Option ((a : α) × β a) :=
-  t.lift (fun m => m.getEntryGE? k) (fun m m' (h : m ~m m') => h.getEntryGE?_eq)
+  t.lift (fun m => m.getEntryGE? k) (fun _ _ h => h.getEntryGE?_eq)
 
 @[inline, inherit_doc DTreeMap.getEntryGT?]
 def getEntryGT? [TransCmp cmp] (t : ExtDTreeMap α β cmp) (k : α) : Option ((a : α) × β a) :=
-  t.lift (fun m => m.getEntryGT? k) (fun m m' (h : m ~m m') => h.getEntryGT?_eq)
+  t.lift (fun m => m.getEntryGT? k) (fun _ _ h => h.getEntryGT?_eq)
 
 @[inline, inherit_doc DTreeMap.getEntryLE?]
 def getEntryLE? [TransCmp cmp] (t : ExtDTreeMap α β cmp) (k : α) : Option ((a : α) × β a) :=
-  t.lift (fun m => m.getEntryLE? k) (fun m m' (h : m ~m m') => h.getEntryLE?_eq)
+  t.lift (fun m => m.getEntryLE? k) (fun _ _ h => h.getEntryLE?_eq)
 
 @[inline, inherit_doc DTreeMap.getEntryLT?]
 def getEntryLT? [TransCmp cmp] (t : ExtDTreeMap α β cmp) (k : α) : Option ((a : α) × β a) :=
-  t.lift (fun m => m.getEntryLT? k) (fun m m' (h : m ~m m') => h.getEntryLT?_eq)
+  t.lift (fun m => m.getEntryLT? k) (fun _ _ h => h.getEntryLT?_eq)
 
 @[inline, inherit_doc DTreeMap.getEntryGE]
 def getEntryGE [TransCmp cmp] (t : ExtDTreeMap α β cmp) (k : α) (h : ∃ a ∈ t, (cmp a k).isGE) :
     (a : α) × β a :=
   t.pliftOn (fun m h' => m.getEntryGE k (h' ▸ h :))
-    (fun m m' _ _ (h : m ~m m') => h.getEntryGE_eq)
+    (fun _ _ _ _ h => h.getEntryGE_eq)
 
 @[inline, inherit_doc DTreeMap.getEntryGT]
 def getEntryGT [TransCmp cmp] (t : ExtDTreeMap α β cmp) (k : α) (h : ∃ a ∈ t, cmp a k = .gt) :
     (a : α) × β a :=
   t.pliftOn (fun m h' => m.getEntryGT k (h' ▸ h :))
-    (fun m m' _ _ (h : m ~m m') => h.getEntryGT_eq)
+    (fun _ _ _ _ h => h.getEntryGT_eq)
 
 @[inline, inherit_doc DTreeMap.getEntryLE]
 def getEntryLE [TransCmp cmp] (t : ExtDTreeMap α β cmp) (k : α) (h : ∃ a ∈ t, (cmp a k).isLE) :
     (a : α) × β a :=
   t.pliftOn (fun m h' => m.getEntryLE k (h' ▸ h :))
-    (fun m m' _ _ (h : m ~m m') => h.getEntryLE_eq)
+    (fun _ _ _ _ h => h.getEntryLE_eq)
 
 @[inline, inherit_doc DTreeMap.getEntryLT]
 def getEntryLT [TransCmp cmp] (t : ExtDTreeMap α β cmp) (k : α) (h : ∃ a ∈ t, cmp a k = .lt) :
     (a : α) × β a :=
   t.pliftOn (fun m h' => m.getEntryLT k (h' ▸ h :))
-    (fun m m' _ _ (h : m ~m m') => h.getEntryLT_eq)
+    (fun _ _ _ _ h => h.getEntryLT_eq)
 
 @[inline, inherit_doc DTreeMap.getEntryGE!]
 def getEntryGE! [TransCmp cmp] [Inhabited (Sigma β)] (t : ExtDTreeMap α β cmp) (k : α) : (a : α) × β a :=
-  t.lift (fun m => m.getEntryGE! k) (fun m m' (h : m ~m m') => h.getEntryGE!_eq)
+  t.lift (fun m => m.getEntryGE! k) (fun _ _ h => h.getEntryGE!_eq)
 
 @[inline, inherit_doc DTreeMap.getEntryGT!]
 def getEntryGT! [TransCmp cmp] [Inhabited (Sigma β)] (t : ExtDTreeMap α β cmp) (k : α) : (a : α) × β a :=
-  t.lift (fun m => m.getEntryGT! k) (fun m m' (h : m ~m m') => h.getEntryGT!_eq)
+  t.lift (fun m => m.getEntryGT! k) (fun _ _ h => h.getEntryGT!_eq)
 
 @[inline, inherit_doc DTreeMap.getEntryLE!]
 def getEntryLE! [TransCmp cmp] [Inhabited (Sigma β)] (t : ExtDTreeMap α β cmp) (k : α) : (a : α) × β a :=
-  t.lift (fun m => m.getEntryLE! k) (fun m m' (h : m ~m m') => h.getEntryLE!_eq)
+  t.lift (fun m => m.getEntryLE! k) (fun _ _ h => h.getEntryLE!_eq)
 
 @[inline, inherit_doc DTreeMap.getEntryLT!]
 def getEntryLT! [TransCmp cmp] [Inhabited (Sigma β)] (t : ExtDTreeMap α β cmp) (k : α) : (a : α) × β a :=
-  t.lift (fun m => m.getEntryLT! k) (fun m m' (h : m ~m m') => h.getEntryLT!_eq)
+  t.lift (fun m => m.getEntryLT! k) (fun _ _ h => h.getEntryLT!_eq)
 
 @[inline, inherit_doc DTreeMap.getEntryGED]
 def getEntryGED [TransCmp cmp] (t : ExtDTreeMap α β cmp) (k : α) (fallback : Sigma β) : (a : α) × β a :=
-  t.lift (fun m => m.getEntryGED k fallback) (fun m m' (h : m ~m m') => h.getEntryGED_eq)
+  t.lift (fun m => m.getEntryGED k fallback) (fun _ _ h => h.getEntryGED_eq)
 
 @[inline, inherit_doc DTreeMap.getEntryGTD]
 def getEntryGTD [TransCmp cmp] (t : ExtDTreeMap α β cmp) (k : α) (fallback : Sigma β) : (a : α) × β a :=
-  t.lift (fun m => m.getEntryGTD k fallback) (fun m m' (h : m ~m m') => h.getEntryGTD_eq)
+  t.lift (fun m => m.getEntryGTD k fallback) (fun _ _ h => h.getEntryGTD_eq)
 
 @[inline, inherit_doc DTreeMap.getEntryLED]
 def getEntryLED [TransCmp cmp] (t : ExtDTreeMap α β cmp) (k : α) (fallback : Sigma β) : (a : α) × β a :=
-  t.lift (fun m => m.getEntryLED k fallback) (fun m m' (h : m ~m m') => h.getEntryLED_eq)
+  t.lift (fun m => m.getEntryLED k fallback) (fun _ _ h => h.getEntryLED_eq)
 
 @[inline, inherit_doc DTreeMap.getEntryLTD]
 def getEntryLTD [TransCmp cmp] (t : ExtDTreeMap α β cmp) (k : α) (fallback : Sigma β) : (a : α) × β a :=
-  t.lift (fun m => m.getEntryLTD k fallback) (fun m m' (h : m ~m m') => h.getEntryLTD_eq)
+  t.lift (fun m => m.getEntryLTD k fallback) (fun _ _ h => h.getEntryLTD_eq)
 
 @[inline, inherit_doc DTreeMap.getKeyGE?]
 def getKeyGE? [TransCmp cmp] (t : ExtDTreeMap α β cmp) (k : α) : Option α :=
-  t.lift (fun m => m.getKeyGE? k) (fun m m' (h : m ~m m') => h.getKeyGE?_eq)
+  t.lift (fun m => m.getKeyGE? k) (fun _ _ h => h.getKeyGE?_eq)
 
 @[inline, inherit_doc DTreeMap.getKeyGT?]
 def getKeyGT? [TransCmp cmp] (t : ExtDTreeMap α β cmp) (k : α) : Option α :=
-  t.lift (fun m => m.getKeyGT? k) (fun m m' (h : m ~m m') => h.getKeyGT?_eq)
+  t.lift (fun m => m.getKeyGT? k) (fun _ _ h => h.getKeyGT?_eq)
 
 @[inline, inherit_doc DTreeMap.getKeyLE?]
 def getKeyLE? [TransCmp cmp] (t : ExtDTreeMap α β cmp) (k : α) : Option α :=
-  t.lift (fun m => m.getKeyLE? k) (fun m m' (h : m ~m m') => h.getKeyLE?_eq)
+  t.lift (fun m => m.getKeyLE? k) (fun _ _ h => h.getKeyLE?_eq)
 
 @[inline, inherit_doc DTreeMap.getKeyLT?]
 def getKeyLT? [TransCmp cmp] (t : ExtDTreeMap α β cmp) (k : α) : Option α :=
-  t.lift (fun m => m.getKeyLT? k) (fun m m' (h : m ~m m') => h.getKeyLT?_eq)
+  t.lift (fun m => m.getKeyLT? k) (fun _ _ h => h.getKeyLT?_eq)
 
 @[inline, inherit_doc DTreeMap.getKeyGE]
 def getKeyGE [TransCmp cmp] (t : ExtDTreeMap α β cmp) (k : α) (h : ∃ a ∈ t, (cmp a k).isGE) : α :=
   t.pliftOn (fun m h' => m.getKeyGE k (h' ▸ h :))
-    (fun m m' _ _ (h : m ~m m') => h.getKeyGE_eq)
+    (fun _ _ _ _ h => h.getKeyGE_eq)
 
 @[inline, inherit_doc DTreeMap.getKeyGT]
 def getKeyGT [TransCmp cmp] (t : ExtDTreeMap α β cmp) (k : α) (h : ∃ a ∈ t, cmp a k = .gt) : α :=
   t.pliftOn (fun m h' => m.getKeyGT k (h' ▸ h :))
-    (fun m m' _ _ (h : m ~m m') => h.getKeyGT_eq)
+    (fun _ _ _ _ h => h.getKeyGT_eq)
 
 @[inline, inherit_doc DTreeMap.getKeyLE]
 def getKeyLE [TransCmp cmp] (t : ExtDTreeMap α β cmp) (k : α) (h : ∃ a ∈ t, (cmp a k).isLE) : α :=
   t.pliftOn (fun m h' => m.getKeyLE k (h' ▸ h :))
-    (fun m m' _ _ (h : m ~m m') => h.getKeyLE_eq)
+    (fun _ _ _ _ h => h.getKeyLE_eq)
 
 @[inline, inherit_doc DTreeMap.getKeyLT]
 def getKeyLT [TransCmp cmp] (t : ExtDTreeMap α β cmp) (k : α) (h : ∃ a ∈ t, cmp a k = .lt) : α :=
   t.pliftOn (fun m h' => m.getKeyLT k (h' ▸ h :))
-    (fun m m' _ _ (h : m ~m m') => h.getKeyLT_eq)
+    (fun _ _ _ _ h => h.getKeyLT_eq)
 
 @[inline, inherit_doc DTreeMap.getKeyGE!]
 def getKeyGE! [TransCmp cmp] [Inhabited α] (t : ExtDTreeMap α β cmp) (k : α) : α :=
-  t.lift (fun m => m.getKeyGE! k) (fun m m' (h : m ~m m') => h.getKeyGE!_eq)
+  t.lift (fun m => m.getKeyGE! k) (fun _ _ h => h.getKeyGE!_eq)
 
 @[inline, inherit_doc DTreeMap.getKeyGT!]
 def getKeyGT! [TransCmp cmp] [Inhabited α] (t : ExtDTreeMap α β cmp) (k : α) : α :=
-  t.lift (fun m => m.getKeyGT! k) (fun m m' (h : m ~m m') => h.getKeyGT!_eq)
+  t.lift (fun m => m.getKeyGT! k) (fun _ _ h => h.getKeyGT!_eq)
 
 @[inline, inherit_doc DTreeMap.getKeyLE!]
 def getKeyLE! [TransCmp cmp] [Inhabited α] (t : ExtDTreeMap α β cmp) (k : α) : α :=
-  t.lift (fun m => m.getKeyLE! k) (fun m m' (h : m ~m m') => h.getKeyLE!_eq)
+  t.lift (fun m => m.getKeyLE! k) (fun _ _ h => h.getKeyLE!_eq)
 
 @[inline, inherit_doc DTreeMap.getKeyLT!]
 def getKeyLT! [TransCmp cmp] [Inhabited α] (t : ExtDTreeMap α β cmp) (k : α) : α :=
-  t.lift (fun m => m.getKeyLT! k) (fun m m' (h : m ~m m') => h.getKeyLT!_eq)
+  t.lift (fun m => m.getKeyLT! k) (fun _ _ h => h.getKeyLT!_eq)
 
 @[inline, inherit_doc DTreeMap.getKeyGED]
 def getKeyGED [TransCmp cmp] (t : ExtDTreeMap α β cmp) (k : α) (fallback : α) : α :=
-  t.lift (fun m => m.getKeyGED k fallback) (fun m m' (h : m ~m m') => h.getKeyGED_eq)
+  t.lift (fun m => m.getKeyGED k fallback) (fun _ _ h => h.getKeyGED_eq)
 
 @[inline, inherit_doc DTreeMap.getKeyGTD]
 def getKeyGTD [TransCmp cmp] (t : ExtDTreeMap α β cmp) (k : α) (fallback : α) : α :=
-  t.lift (fun m => m.getKeyGTD k fallback) (fun m m' (h : m ~m m') => h.getKeyGTD_eq)
+  t.lift (fun m => m.getKeyGTD k fallback) (fun _ _ h => h.getKeyGTD_eq)
 
 @[inline, inherit_doc DTreeMap.getKeyLED]
 def getKeyLED [TransCmp cmp] (t : ExtDTreeMap α β cmp) (k : α) (fallback : α) : α :=
-  t.lift (fun m => m.getKeyLED k fallback) (fun m m' (h : m ~m m') => h.getKeyLED_eq)
+  t.lift (fun m => m.getKeyLED k fallback) (fun _ _ h => h.getKeyLED_eq)
 
 @[inline, inherit_doc DTreeMap.getKeyLTD]
 def getKeyLTD [TransCmp cmp] (t : ExtDTreeMap α β cmp) (k : α) (fallback : α) : α :=
-  t.lift (fun m => m.getKeyLTD k fallback) (fun m m' (h : m ~m m') => h.getKeyLTD_eq)
+  t.lift (fun m => m.getKeyLTD k fallback) (fun _ _ h => h.getKeyLTD_eq)
 
 namespace Const
 
@@ -455,13 +491,13 @@ variable {β : Type v}
 @[inline, inherit_doc ExtDTreeMap.getThenInsertIfNew?]
 def getThenInsertIfNew? [TransCmp cmp] (t : ExtDTreeMap α β cmp) (a : α) (b : β) :
     Option β × ExtDTreeMap α β cmp :=
-  t.lift (fun m => let m' := DTreeMap.Const.getThenInsertIfNew? m a b; (m'.1, Quotient.mk' m'.2))
-    (fun m m' (h : m ~m m') =>
+  t.lift (fun m => let m' := DTreeMap.Const.getThenInsertIfNew? m a b; (m'.1, mk m'.2))
+    (fun m m' h =>
       Prod.ext
         ((DTreeMap.Const.getThenInsertIfNew?_fst (t := m)).symm ▸
           (DTreeMap.Const.getThenInsertIfNew?_fst (t := m')).symm ▸
           h.constGet?_eq)
-        (Quotient.sound <|
+        (sound <|
           (DTreeMap.Const.getThenInsertIfNew?_snd (t := m)).symm ▸
           (DTreeMap.Const.getThenInsertIfNew?_snd (t := m')).symm ▸
           h.insertIfNew a b))
@@ -469,167 +505,167 @@ def getThenInsertIfNew? [TransCmp cmp] (t : ExtDTreeMap α β cmp) (a : α) (b :
 @[inline, inherit_doc ExtDTreeMap.get?]
 def get? [TransCmp cmp] (t : ExtDTreeMap α β cmp) (a : α) : Option β :=
   t.lift (fun m => DTreeMap.Const.get? m a)
-    (fun m m' (h : m ~m m') => h.constGet?_eq)
+    (fun _ _ h => h.constGet?_eq)
 
 @[inline, inherit_doc ExtDTreeMap.get]
 def get [TransCmp cmp] (t : ExtDTreeMap α β cmp) (a : α) (h : a ∈ t) : β :=
   t.pliftOn (fun m h' => DTreeMap.Const.get m a (h' ▸ h :))
-    (fun m m' _ _ (h : m ~m m') => h.constGet_eq)
+    (fun _ _ _ _ h => h.constGet_eq)
 
 @[inline, inherit_doc ExtDTreeMap.get!]
 def get! [TransCmp cmp] (t : ExtDTreeMap α β cmp) (a : α) [Inhabited β] : β :=
   t.lift (fun m => DTreeMap.Const.get! m a)
-    (fun m m' (h : m ~m m') => h.constGet!_eq)
+    (fun _ _ h => h.constGet!_eq)
 
 @[inline, inherit_doc ExtDTreeMap.getD]
 def getD [TransCmp cmp] (t : ExtDTreeMap α β cmp) (a : α) (fallback : β) : β :=
   t.lift (fun m => DTreeMap.Const.getD m a fallback)
-    (fun m m' (h : m ~m m') => h.constGetD_eq)
+    (fun _ _ h => h.constGetD_eq)
 
 @[inline, inherit_doc ExtDTreeMap.minEntry?]
 def minEntry? [TransCmp cmp] (t : ExtDTreeMap α β cmp) : Option (α × β) :=
   t.lift (fun m => DTreeMap.Const.minEntry? m)
-    (fun m m' (h : m ~m m') => h.constMinEntry?_eq)
+    (fun _ _ h => h.constMinEntry?_eq)
 
 @[inline, inherit_doc ExtDTreeMap.minEntry]
 def minEntry [TransCmp cmp] (t : ExtDTreeMap α β cmp) (h : t ≠ ∅) : α × β :=
   t.pliftOn (fun m h' => DTreeMap.Const.minEntry m (h' ▸ isEmpty_eq_false_iff.mpr h :))
-    (fun m m' _ _ (h : m ~m m') => h.constMinEntry_eq)
+    (fun _ _ _ _ h => h.constMinEntry_eq)
 
 @[inline, inherit_doc ExtDTreeMap.minEntry!]
 def minEntry! [TransCmp cmp] [Inhabited (α × β)] (t : ExtDTreeMap α β cmp) : α × β :=
   t.lift (fun m => DTreeMap.Const.minEntry! m)
-    (fun m m' (h : m ~m m') => h.constMinEntry!_eq)
+    (fun _ _ h => h.constMinEntry!_eq)
 
 @[inline, inherit_doc ExtDTreeMap.minEntryD]
 def minEntryD [TransCmp cmp] (t : ExtDTreeMap α β cmp) (fallback : α × β) : α × β :=
   t.lift (fun m => DTreeMap.Const.minEntryD m fallback)
-    (fun m m' (h : m ~m m') => h.constMinEntryD_eq)
+    (fun _ _ h => h.constMinEntryD_eq)
 
 @[inline, inherit_doc ExtDTreeMap.maxEntry?]
 def maxEntry? [TransCmp cmp] (t : ExtDTreeMap α β cmp) : Option (α × β) :=
   t.lift (fun m => DTreeMap.Const.maxEntry? m)
-    (fun m m' (h : m ~m m') => h.constMaxEntry?_eq)
+    (fun _ _ h => h.constMaxEntry?_eq)
 
 @[inline, inherit_doc ExtDTreeMap.maxEntry]
 def maxEntry [TransCmp cmp] (t : ExtDTreeMap α β cmp) (h : t ≠ ∅) : α × β :=
   t.pliftOn (fun m h' => DTreeMap.Const.maxEntry m (h' ▸ isEmpty_eq_false_iff.mpr h :))
-    (fun m m' _ _ (h : m ~m m') => h.constMaxEntry_eq)
+    (fun _ _ _ _ h => h.constMaxEntry_eq)
 
 @[inline, inherit_doc ExtDTreeMap.maxEntry!]
 def maxEntry! [TransCmp cmp] [Inhabited (α × β)] (t : ExtDTreeMap α β cmp) : α × β :=
   t.lift (fun m => DTreeMap.Const.maxEntry! m)
-    (fun m m' (h : m ~m m') => h.constMaxEntry!_eq)
+    (fun _ _ h => h.constMaxEntry!_eq)
 
 @[inline, inherit_doc ExtDTreeMap.maxEntryD]
 def maxEntryD [TransCmp cmp] (t : ExtDTreeMap α β cmp) (fallback : α × β) : α × β :=
   t.lift (fun m => DTreeMap.Const.maxEntryD m fallback)
-    (fun m m' (h : m ~m m') => h.constMaxEntryD_eq)
+    (fun _ _ h => h.constMaxEntryD_eq)
 
 @[inline, inherit_doc ExtDTreeMap.entryAtIdx?]
 def entryAtIdx? [TransCmp cmp] (t : ExtDTreeMap α β cmp) (n : Nat) : Option (α × β) :=
   t.lift (fun m => DTreeMap.Const.entryAtIdx? m n)
-    (fun m m' (h : m ~m m') => h.constEntryAtIdx?_eq)
+    (fun _ _ h => h.constEntryAtIdx?_eq)
 
 @[inline, inherit_doc ExtDTreeMap.entryAtIdx]
 def entryAtIdx [TransCmp cmp] (t : ExtDTreeMap α β cmp) (n : Nat) (h : n < t.size) : α × β :=
   t.pliftOn (fun m h' => DTreeMap.Const.entryAtIdx m n (h' ▸ h :))
-    (fun m m' _ _ (h : m ~m m') => h.constEntryAtIdx_eq)
+    (fun _ _ _ _ h => h.constEntryAtIdx_eq)
 
 @[inline, inherit_doc ExtDTreeMap.entryAtIdx!]
 def entryAtIdx! [TransCmp cmp] [Inhabited (α × β)] (t : ExtDTreeMap α β cmp) (n : Nat) : α × β :=
   t.lift (fun m => DTreeMap.Const.entryAtIdx! m n)
-    (fun m m' (h : m ~m m') => h.constEntryAtIdx!_eq)
+    (fun _ _ h => h.constEntryAtIdx!_eq)
 
 @[inline, inherit_doc ExtDTreeMap.entryAtIdxD]
 def entryAtIdxD [TransCmp cmp] (t : ExtDTreeMap α β cmp) (n : Nat)
     (fallback : α × β) : α × β :=
   t.lift (fun m => DTreeMap.Const.entryAtIdxD m n fallback)
-    (fun m m' (h : m ~m m') => h.constEntryAtIdxD_eq)
+    (fun _ _ h => h.constEntryAtIdxD_eq)
 
 @[inline, inherit_doc ExtDTreeMap.getEntryGE?]
 def getEntryGE? [TransCmp cmp] (t : ExtDTreeMap α β cmp) (k : α) : Option (α × β) :=
   t.lift (fun m => DTreeMap.Const.getEntryGE? m k)
-    (fun m m' (h : m ~m m') => h.constGetEntryGE?_eq)
+    (fun _ _ h => h.constGetEntryGE?_eq)
 
 @[inline, inherit_doc ExtDTreeMap.getEntryGT?]
 def getEntryGT? [TransCmp cmp] (t : ExtDTreeMap α β cmp) (k : α) : Option (α × β) :=
   t.lift (fun m => DTreeMap.Const.getEntryGT? m k)
-    (fun m m' (h : m ~m m') => h.constGetEntryGT?_eq)
+    (fun _ _ h => h.constGetEntryGT?_eq)
 
 @[inline, inherit_doc ExtDTreeMap.getEntryLE?]
 def getEntryLE? [TransCmp cmp] (t : ExtDTreeMap α β cmp) (k : α) : Option (α × β) :=
   t.lift (fun m => DTreeMap.Const.getEntryLE? m k)
-    (fun m m' (h : m ~m m') => h.constGetEntryLE?_eq)
+    (fun _ _ h => h.constGetEntryLE?_eq)
 
 @[inline, inherit_doc ExtDTreeMap.getEntryLT?]
 def getEntryLT? [TransCmp cmp] (t : ExtDTreeMap α β cmp) (k : α) : Option (α × β) :=
   t.lift (fun m => DTreeMap.Const.getEntryLT? m k)
-    (fun m m' (h : m ~m m') => h.constGetEntryLT?_eq)
+    (fun _ _ h => h.constGetEntryLT?_eq)
 
 @[inline, inherit_doc ExtDTreeMap.getEntryGE]
 def getEntryGE [TransCmp cmp] (t : ExtDTreeMap α β cmp) (k : α) (h : ∃ a ∈ t, (cmp a k).isGE) :
     α × β :=
   t.pliftOn (fun m h' => DTreeMap.Const.getEntryGE m k (h' ▸ h :))
-    (fun m m' _ _ (h : m ~m m') => h.constGetEntryGE_eq)
+    (fun _ _ _ _ h => h.constGetEntryGE_eq)
 
 @[inline, inherit_doc ExtDTreeMap.getEntryGT]
 def getEntryGT [TransCmp cmp] (t : ExtDTreeMap α β cmp) (k : α) (h : ∃ a ∈ t, cmp a k = .gt) :
     α × β :=
   t.pliftOn (fun m h' => DTreeMap.Const.getEntryGT m k (h' ▸ h :))
-    (fun m m' _ _ (h : m ~m m') => h.constGetEntryGT_eq)
+    (fun _ _ _ _ h => h.constGetEntryGT_eq)
 
 @[inline, inherit_doc ExtDTreeMap.getEntryLE]
 def getEntryLE [TransCmp cmp] (t : ExtDTreeMap α β cmp) (k : α) (h : ∃ a ∈ t, (cmp a k).isLE) :
     α × β :=
   t.pliftOn (fun m h' => DTreeMap.Const.getEntryLE m k (h' ▸ h :))
-    (fun m m' _ _ (h : m ~m m') => h.constGetEntryLE_eq)
+    (fun _ _ _ _ h => h.constGetEntryLE_eq)
 
 @[inline, inherit_doc ExtDTreeMap.getEntryLT]
 def getEntryLT [TransCmp cmp] (t : ExtDTreeMap α β cmp) (k : α) (h : ∃ a ∈ t, cmp a k = .lt) :
     α × β :=
   t.pliftOn (fun m h' => DTreeMap.Const.getEntryLT m k (h' ▸ h :))
-    (fun m m' _ _ (h : m ~m m') => h.constGetEntryLT_eq)
+    (fun _ _ _ _ h => h.constGetEntryLT_eq)
 
 @[inline, inherit_doc ExtDTreeMap.getEntryGE!]
 def getEntryGE! [TransCmp cmp] [Inhabited (α × β)] (t : ExtDTreeMap α β cmp) (k : α) : (α × β) :=
   t.lift (fun m => DTreeMap.Const.getEntryGE! m k)
-    (fun m m' (h : m ~m m') => h.constGetEntryGE!_eq)
+    (fun _ _ h => h.constGetEntryGE!_eq)
 
 @[inline, inherit_doc ExtDTreeMap.getEntryGT!]
 def getEntryGT! [TransCmp cmp] [Inhabited (α × β)] (t : ExtDTreeMap α β cmp) (k : α) : (α × β) :=
   t.lift (fun m => DTreeMap.Const.getEntryGT! m k)
-    (fun m m' (h : m ~m m') => h.constGetEntryGT!_eq)
+    (fun _ _ h => h.constGetEntryGT!_eq)
 
 @[inline, inherit_doc ExtDTreeMap.getEntryLE!]
 def getEntryLE! [TransCmp cmp] [Inhabited (α × β)] (t : ExtDTreeMap α β cmp) (k : α) : (α × β) :=
   t.lift (fun m => DTreeMap.Const.getEntryLE! m k)
-    (fun m m' (h : m ~m m') => h.constGetEntryLE!_eq)
+    (fun _ _ h => h.constGetEntryLE!_eq)
 
 @[inline, inherit_doc ExtDTreeMap.getEntryLT!]
 def getEntryLT! [TransCmp cmp] [Inhabited (α × β)] (t : ExtDTreeMap α β cmp) (k : α) : (α × β) :=
   t.lift (fun m => DTreeMap.Const.getEntryLT! m k)
-    (fun m m' (h : m ~m m') => h.constGetEntryLT!_eq)
+    (fun _ _ h => h.constGetEntryLT!_eq)
 
 @[inline, inherit_doc ExtDTreeMap.getEntryGED]
 def getEntryGED [TransCmp cmp] (t : ExtDTreeMap α β cmp) (k : α) (fallback : α × β) : (α × β) :=
   t.lift (fun m => DTreeMap.Const.getEntryGED m k fallback)
-    (fun m m' (h : m ~m m') => h.constGetEntryGED_eq)
+    (fun _ _ h => h.constGetEntryGED_eq)
 
 @[inline, inherit_doc ExtDTreeMap.getEntryGTD]
 def getEntryGTD [TransCmp cmp] (t : ExtDTreeMap α β cmp) (k : α) (fallback : α × β) : (α × β) :=
   t.lift (fun m => DTreeMap.Const.getEntryGTD m k fallback)
-    (fun m m' (h : m ~m m') => h.constGetEntryGTD_eq)
+    (fun _ _ h => h.constGetEntryGTD_eq)
 
 @[inline, inherit_doc ExtDTreeMap.getEntryLED]
 def getEntryLED [TransCmp cmp] (t : ExtDTreeMap α β cmp) (k : α) (fallback : α × β) : (α × β) :=
   t.lift (fun m => DTreeMap.Const.getEntryLED m k fallback)
-    (fun m m' (h : m ~m m') => h.constGetEntryLED_eq)
+    (fun _ _ h => h.constGetEntryLED_eq)
 
 @[inline, inherit_doc ExtDTreeMap.getEntryLTD]
 def getEntryLTD [TransCmp cmp] (t : ExtDTreeMap α β cmp) (k : α) (fallback : α × β) : (α × β) :=
   t.lift (fun m => DTreeMap.Const.getEntryLTD m k fallback)
-    (fun m m' (h : m ~m m') => h.constGetEntryLTD_eq)
+    (fun _ _ h => h.constGetEntryLTD_eq)
 
 end Const
 
@@ -637,34 +673,34 @@ variable {δ : Type w} {m : Type w → Type w₂} [Monad m] [LawfulMonad m]
 
 @[inline, inherit_doc DTreeMap.filter]
 def filter (f : (a : α) → β a → Bool) (t : ExtDTreeMap α β cmp) : ExtDTreeMap α β cmp :=
-  t.lift (fun m => Quotient.mk' (m.filter f))
-    (fun m m' (h : m ~m m') => Quotient.sound (h.filter f))
+  t.lift (fun m => mk (m.filter f))
+    (fun _ _ h => sound (h.filter f))
 
 @[inline, inherit_doc DTreeMap.filterMap]
 def filterMap (f : (a : α) → β a → Option (γ a)) (t : ExtDTreeMap α β cmp) : ExtDTreeMap α γ cmp :=
-  t.lift (fun m => Quotient.mk' (m.filterMap f))
-    (fun m m' (h : m ~m m') => Quotient.sound (h.filterMap f))
+  t.lift (fun m => mk (m.filterMap f))
+    (fun _ _ h => sound (h.filterMap f))
 
 @[inline, inherit_doc DTreeMap.map]
 def map (f : (a : α) → β a → γ a) (t : ExtDTreeMap α β cmp) : ExtDTreeMap α γ cmp :=
-  t.lift (fun m => Quotient.mk' (m.map f))
-    (fun m m' (h : m ~m m') => Quotient.sound (h.map f))
+  t.lift (fun m => mk (m.map f))
+    (fun _ _ h => sound (h.map f))
 
 @[inline, inherit_doc DTreeMap.foldlM]
 def foldlM [TransCmp cmp] (f : δ → (a : α) → β a → m δ) (init : δ) (t : ExtDTreeMap α β cmp) : m δ :=
-  t.lift (fun m => m.foldlM f init) (fun m m' (h : m ~m m') => h.foldlM_eq)
+  t.lift (fun m => m.foldlM f init) (fun _ _ h => h.foldlM_eq)
 
 @[inline, inherit_doc DTreeMap.foldl]
 def foldl [TransCmp cmp] (f : δ → (a : α) → β a → δ) (init : δ) (t : ExtDTreeMap α β cmp) : δ :=
-  t.lift (fun m => m.foldl f init) (fun m m' (h : m ~m m') => h.foldl_eq)
+  t.lift (fun m => m.foldl f init) (fun _ _ h => h.foldl_eq)
 
 @[inline, inherit_doc DTreeMap.foldrM]
 def foldrM [TransCmp cmp] (f : (a : α) → β a → δ → m δ) (init : δ) (t : ExtDTreeMap α β cmp) : m δ :=
-  t.lift (fun m => m.foldrM f init) (fun m m' (h : m ~m m') => h.foldrM_eq)
+  t.lift (fun m => m.foldrM f init) (fun _ _ h => h.foldrM_eq)
 
 @[inline, inherit_doc DTreeMap.foldr]
 def foldr [TransCmp cmp] (f : (a : α) → β a → δ → δ) (init : δ) (t : ExtDTreeMap α β cmp) : δ :=
-  t.lift (fun m => m.foldr f init) (fun m m' (h : m ~m m') => h.foldr_eq)
+  t.lift (fun m => m.foldr f init) (fun _ _ h => h.foldr_eq)
 
 @[inline, inherit_doc DTreeMap.partition]
 def partition [TransCmp cmp] (f : (a : α) → β a → Bool)
@@ -677,11 +713,11 @@ def partition [TransCmp cmp] (f : (a : α) → β a → Bool)
 
 @[inline, inherit_doc DTreeMap.forM]
 def forM [TransCmp cmp] (f : (a : α) → β a → m PUnit) (t : ExtDTreeMap α β cmp) : m PUnit :=
-  t.lift (fun m => m.forM f) (fun m m' (h : m ~m m') => h.forM_eq (f := fun x => f x.1 x.2))
+  t.lift (fun m => m.forM f) (fun _ _ h => h.forM_eq (f := fun x => f x.1 x.2))
 
 @[inline, inherit_doc DTreeMap.forIn]
 def forIn [TransCmp cmp] (f : (a : α) → β a → δ → m (ForInStep δ)) (init : δ) (t : ExtDTreeMap α β cmp) : m δ :=
-  t.lift (fun m => m.forIn f init) (fun m m' (h : m ~m m') => h.forIn_eq (f := fun x => f x.1 x.2))
+  t.lift (fun m => m.forIn f init) (fun _ _ h => h.forIn_eq (f := fun x => f x.1 x.2))
 
 /-
 Note: We ignore the monad instance provided by `forM` / `forIn` and instead use the one from the
@@ -716,63 +752,63 @@ end Const
 
 @[inline, inherit_doc DTreeMap.any]
 def any [TransCmp cmp] (t : ExtDTreeMap α β cmp) (p : (a : α) → β a → Bool) : Bool :=
-  t.lift (fun m => m.any p) (fun m m' (h : m ~m m') => h.any_eq)
+  t.lift (fun m => m.any p) (fun _ _ h => h.any_eq)
 
 @[inline, inherit_doc DTreeMap.all]
 def all [TransCmp cmp] (t : ExtDTreeMap α β cmp) (p : (a : α) → β a → Bool) : Bool :=
-  t.lift (fun m => m.all p) (fun m m' (h : m ~m m') => h.all_eq)
+  t.lift (fun m => m.all p) (fun _ _ h => h.all_eq)
 
 @[inline, inherit_doc DTreeMap.keys]
 def keys [TransCmp cmp] (t : ExtDTreeMap α β cmp) : List α :=
-  t.lift (fun m => m.keys) (fun m m' (h : m ~m m') => h.keys_eq)
+  t.lift (fun m => m.keys) (fun _ _ h => h.keys_eq)
 
 @[inline, inherit_doc DTreeMap.keysArray]
 def keysArray [TransCmp cmp] (t : ExtDTreeMap α β cmp) : Array α :=
-  t.lift (fun m => m.keysArray) (fun m m' (h : m ~m m') => h.keysArray_eq)
+  t.lift (fun m => m.keysArray) (fun _ _ h => h.keysArray_eq)
 
 @[inline, inherit_doc DTreeMap.values]
 def values [TransCmp cmp] {β : Type v} (t : ExtDTreeMap α β cmp) : List β :=
-  t.lift (fun m => m.values) (fun m m' (h : m ~m m') => h.values_eq)
+  t.lift (fun m => m.values) (fun _ _ h => h.values_eq)
 
 @[inline, inherit_doc DTreeMap.valuesArray]
 def valuesArray [TransCmp cmp] {β : Type v} (t : ExtDTreeMap α β cmp) : Array β :=
-  t.lift (fun m => m.valuesArray) (fun m m' (h : m ~m m') => h.valuesArray_eq)
+  t.lift (fun m => m.valuesArray) (fun _ _ h => h.valuesArray_eq)
 
 @[inline, inherit_doc DTreeMap.toList]
 def toList [TransCmp cmp] (t : ExtDTreeMap α β cmp) : List ((a : α) × β a) :=
-  t.lift (fun m => m.toList) (fun m m' (h : m ~m m') => h.toList_eq)
+  t.lift (fun m => m.toList) (fun _ _ h => h.toList_eq)
 
 @[inline, inherit_doc DTreeMap.ofList]
 def ofList (l : List ((a : α) × β a)) (cmp : α → α → Ordering := by exact compare) :
     ExtDTreeMap α β cmp :=
-  Quotient.mk' (.ofList l cmp)
+  mk (.ofList l cmp)
 
 @[inline, inherit_doc DTreeMap.toArray]
 def toArray [TransCmp cmp] (t : ExtDTreeMap α β cmp) : Array ((a : α) × β a) :=
-  t.lift (fun m => m.toArray) (fun m m' (h : m ~m m') => h.toArray_eq)
+  t.lift (fun m => m.toArray) (fun _ _ h => h.toArray_eq)
 
 @[inline, inherit_doc DTreeMap.ofArray]
 def ofArray (a : Array ((a : α) × β a)) (cmp : α → α → Ordering := by exact compare) :
     ExtDTreeMap α β cmp :=
-  Quotient.mk' (.ofArray a cmp)
+  mk (.ofArray a cmp)
 
 @[inline, inherit_doc DTreeMap.modify]
 def modify [TransCmp cmp] [LawfulEqCmp cmp] (t : ExtDTreeMap α β cmp) (a : α) (f : β a → β a) :
     ExtDTreeMap α β cmp :=
-  t.lift (fun m => Quotient.mk' (m.modify a f))
-    (fun m m' (h : m ~m m') => Quotient.sound (h.modify a f))
+  t.lift (fun m => mk (m.modify a f))
+    (fun _ _ h => sound (h.modify a f))
 
 @[inline, inherit_doc DTreeMap.alter]
 def alter [TransCmp cmp] [LawfulEqCmp cmp] (t : ExtDTreeMap α β cmp) (a : α) (f : Option (β a) → Option (β a)) :
     ExtDTreeMap α β cmp :=
-  t.lift (fun m => Quotient.mk' (m.alter a f))
-    (fun m m' (h : m ~m m') => Quotient.sound (h.alter a f))
+  t.lift (fun m => mk (m.alter a f))
+    (fun _ _ h => sound (h.alter a f))
 
 @[inline, inherit_doc DTreeMap.mergeWith]
 def mergeWith [TransCmp cmp] [LawfulEqCmp cmp] (mergeFn : (a : α) → β a → β a → β a) (t₁ t₂ : ExtDTreeMap α β cmp) :
     ExtDTreeMap α β cmp :=
-  t₁.liftOn₂ t₂ (fun m₁ m₂ => Quotient.mk' (m₁.mergeWith mergeFn m₂))
-    (fun m₁ m₂ m₁' m₂' (h₁ : m₁ ~m m₁') (h₂ : m₂ ~m m₂') => Quotient.sound (h₁.mergeWith mergeFn h₂))
+  t₁.liftOn₂ t₂ (fun m₁ m₂ => mk (m₁.mergeWith mergeFn m₂))
+    (fun _ _ _ _ h₁ h₂ => sound (h₁.mergeWith mergeFn h₂))
 
 namespace Const
 
@@ -781,43 +817,43 @@ variable {β : Type v}
 @[inline, inherit_doc ExtDTreeMap.toList]
 def toList [TransCmp cmp] (t : ExtDTreeMap α β cmp) : List (α × β) :=
   t.lift (fun m => DTreeMap.Const.toList m)
-    (fun m m' (h : m ~m m') => h.constToList_eq)
+    (fun _ _ h => h.constToList_eq)
 
 @[inline, inherit_doc ExtDTreeMap.ofList]
 def ofList (l : List (α × β)) (cmp : α → α → Ordering := by exact compare) : ExtDTreeMap α β cmp :=
-  Quotient.mk' (DTreeMap.Const.ofList l cmp)
+  mk (DTreeMap.Const.ofList l cmp)
 
 @[inline, inherit_doc ExtDTreeMap.toArray]
 def toArray [TransCmp cmp] (t : ExtDTreeMap α β cmp) : Array (α × β) :=
   t.lift (fun m => DTreeMap.Const.toArray m)
-    (fun m m' (h : m ~m m') => h.constToArray_eq)
+    (fun _ _ h => h.constToArray_eq)
 
 @[inline, inherit_doc ExtDTreeMap.ofList]
 def ofArray (a : Array (α × β)) (cmp : α → α → Ordering := by exact compare) : ExtDTreeMap α β cmp :=
-  Quotient.mk' (DTreeMap.Const.ofArray a cmp)
+  mk (DTreeMap.Const.ofArray a cmp)
 
 @[inline, inherit_doc DTreeMap.Const.unitOfList]
 def unitOfList (l : List α) (cmp : α → α → Ordering := by exact compare) : ExtDTreeMap α Unit cmp :=
-  Quotient.mk' (DTreeMap.Const.unitOfList l cmp)
+  mk (DTreeMap.Const.unitOfList l cmp)
 
 @[inline, inherit_doc DTreeMap.Const.unitOfArray]
 def unitOfArray (a : Array α) (cmp : α → α → Ordering := by exact compare) : ExtDTreeMap α Unit cmp :=
-  Quotient.mk' (DTreeMap.Const.unitOfArray a cmp)
+  mk (DTreeMap.Const.unitOfArray a cmp)
 
 @[inline, inherit_doc ExtDTreeMap.modify]
 def modify [TransCmp cmp] (t : ExtDTreeMap α β cmp) (a : α) (f : β → β) : ExtDTreeMap α β cmp :=
-  t.lift (fun m => Quotient.mk' (DTreeMap.Const.modify m a f))
-    (fun m m' (h : m ~m m') => Quotient.sound (h.constModify a f))
+  t.lift (fun m => mk (DTreeMap.Const.modify m a f))
+    (fun _ _ h => sound (h.constModify a f))
 
 @[inline, inherit_doc ExtDTreeMap.alter]
 def alter [TransCmp cmp] (t : ExtDTreeMap α β cmp) (a : α) (f : Option β → Option β) : ExtDTreeMap α β cmp :=
-  t.lift (fun m => Quotient.mk' (DTreeMap.Const.alter m a f))
-    (fun m m' (h : m ~m m') => Quotient.sound (h.constAlter a f))
+  t.lift (fun m => mk (DTreeMap.Const.alter m a f))
+    (fun _ _ h => sound (h.constAlter a f))
 
 @[inline, inherit_doc ExtDTreeMap.mergeWith]
 def mergeWith [TransCmp cmp] (mergeFn : α → β → β → β) (t₁ t₂ : ExtDTreeMap α β cmp) : ExtDTreeMap α β cmp :=
-  t₁.liftOn₂ t₂ (fun m₁ m₂ => Quotient.mk' (DTreeMap.Const.mergeWith mergeFn m₁ m₂))
-    (fun m₁ m₂ m₁' m₂' (h₁ : m₁ ~m m₁') (h₂ : m₂ ~m m₂') => Quotient.sound (h₁.constMergeWith mergeFn h₂))
+  t₁.liftOn₂ t₂ (fun m₁ m₂ => mk (DTreeMap.Const.mergeWith mergeFn m₁ m₂))
+    (fun _ _ _ _ h₁ h₂ => sound (h₁.constMergeWith mergeFn h₂))
 
 end Const
 
